having a lot of issues with NLarith

concurrency/hack-hash-table/CapacityAllocator.dfy
@@ -49,56 +49,89 @@ module CapacityAllocator {
     Splitted(r', ri)
   }
 
+  function AllowedSize(): (s: nat)
+    ensures 0 < s < FixedSize()
+
+  function method AllowedSizeImpl(): (s: uint32)
+    ensures s as nat == AllowedSize()
+    
   predicate CapPreInit(s: HTResource.R) {
     && s.R?
     && s.table == unitTable()
-    && s.insert_capacity == FixedSize() - 1
+    && s.insert_capacity == AllowedSize()
     && s.tickets == multiset{}
     && s.stubs == multiset{}
+  }
+
+  lemma test(a: nat, b: nat, q: nat, r: nat)
+    requires b >= 1
+    requires q == a / b
+    requires r == a % b
+
+    ensures r + q <= a;
+  {
+    assert a == q * b + r; 
+    assert r + q <= a;
   }
 
   method init(linear in_r: ARS.R)
   returns (mt: AllocatorMutexTable, linear out_r: ARS.R)
   requires CapPreInit(in_r)
-  ensures Inv(mt)
+  // ensures Inv(mt)
   // ensures out_r == unit()
   {
     linear var remaining_r := in_r;
+
+    var total_amount :uint32 := AllowedSizeImpl();
+    var bin_count := BinCountImpl();
     mt := [];
 
+    var quotient :uint32 := total_amount / bin_count;
+    var reaminder :uint32 := total_amount % bin_count;
+    test(total_amount as nat, bin_count as nat, quotient as nat, reaminder as nat);
+
+    var allocated_sum: nat := 0;
     var i: uint32 := 0;
-    var quotient: uint32 := FixedSizeImpl() / BinCountImpl();
-    // var remainder: uint32 := FixedSizeImpl() % BinCountImpl();
-    var allocated_amount :uint32 := 0;
-    var unallocated_amount :uint32 := FixedSizeImpl() - 1;
 
-    while i < BinCountImpl()
-      invariant i as int == |mt| <= BinCount()
-      invariant forall j:nat | j < i as int :: mt[j].inv == BinInv
-      invariant remaining_r.R?
-      invariant remaining_r.insert_capacity == unallocated_amount as int
-      invariant unallocated_amount as nat + allocated_amount as nat == FixedSizeImpl() as nat - 1
-      invariant remaining_r.table == unitTable()
-      invariant remaining_r.tickets == multiset{}
-      invariant remaining_r.stubs == multiset{}
+    while i < bin_count
+      invariant i == 0 ==> allocated_sum == 0;
+      invariant i > 0 ==> (allocated_sum == quotient as nat * i as nat + reaminder as nat);
+      invariant allocated_sum <= total_amount as nat;
+
+      // invariant i as int == |mt| <= BinCount()
+      // invariant forall j:nat | j < i as int :: mt[j].inv == BinInv
+      // invariant remaining_r.R?
+      // invariant remaining_r.insert_capacity == total_amount as nat - allocated_sum
+      // invariant remaining_r.table == unitTable()
+      // invariant remaining_r.tickets == multiset{}
+      // invariant remaining_r.stubs == multiset{}
     {
-      var amount := if unallocated_amount < quotient then unallocated_amount else quotient;
+      var amount := if i == 0 then quotient + reaminder else quotient;
+      allocated_sum := allocated_sum + amount as nat;
 
-      ghost var splitted := Split(remaining_r, amount as nat);
-      linear var ri;
-      remaining_r, ri := ARS.split(remaining_r, splitted.r', splitted.ri);
-      var m := new_mutex(AllocatorBin(amount, ri), BinInv);
-  
-      allocated_amount := allocated_amount + amount;
-      unallocated_amount := unallocated_amount - amount;
-      mt := mt + [m];
+      // ghost var splitted := Split(remaining_r, amount as nat);
+      // linear var ri;
+      // remaining_r, ri := ARS.split(remaining_r, splitted.r', splitted.ri);
+      // var m := new_mutex(AllocatorBin(amount, ri), BinInv);
+      // mt := mt + [m];
+
       i := i + 1;
 
-
-    }
+      assert allocated_sum <= total_amount as nat by {
+        calc <=
+        {
+          allocated_sum;
+          quotient as nat * i as nat + reaminder as nat;
+          {
+            assert i <= bin_count;
+          }
+          quotient as nat * bin_count as nat + reaminder as nat;
+          total_amount as nat;
+        }
+      }
+    } 
 
     out_r := remaining_r;
-    // assert out_r == unit();
   }
 }
 
